\documentclass[12pt]{article}
\usepackage[margin=1in]{geometry}
\usepackage{amsmath}

\pagenumbering{gobble}

\begin{document}
\noindent
Before diving into the solution, let us first focus on the resulting expression from the analysis in \eqref{eq:sample_average}.
\begin{equation}
    \tag{2.6}
    \label{eq:sample_average}
    Q_{n + 1} = \underbrace{\left(1 - \alpha\right)^nQ_1}_\text{initial bias} + \underbrace{\sum^n_{i = 1} \overbrace{\alpha\left(1 - \alpha\right)^{n - i}}^\text{exponential decay}R_i}_\text{weighted average}
    \quad\text{.}
\end{equation}
From the equation, we can see that we need to find an expression for $Q_n$ that contains a recency-weighted average similar to $\sum^n_{i = 1}\alpha\left(1 - \alpha\right)^{n - i}R_i$ but that does not contain an initial bias.
\par\bigskip

\noindent
Let us start by rewriting the incremental average expression for $Q_{n + 1}$.
To keep the notation less cluttered, we will use the following notation: $Q_n \equiv Q_n(a)$ and $R_n \equiv R_n(a)$.
\begin{equation*}
    Q_{n + 1} = Q_n + \beta_n\left[R_n - Q_n\right]
\end{equation*}
Now let's substitute $\beta_n$ into the equation and rearrange a little.
\begin{alignat*}{3}
    & Q_{n + 1} && = Q_n + \beta_n\left[R_n - Q_n\right] \\
    & && = \beta_n R_n + \left(1 - \beta_n\right) Q_n \\
    \implies\quad & Q_{n + 1} && = \left(\frac{\alpha}{\bar{o}_n}\right) R_n + \left(1 - \frac{\alpha}{\bar{o}_n}\right) Q_n \\
    \implies\quad & \bar{o}_n Q_{n + 1} && = \alpha R_n + \bar{o}_n Q_n - \alpha Q_n \\
    & && = \alpha R_n + \left(\bar{o}_n - \alpha\right) Q_n
\end{alignat*}
Now we can substitute in the expression for $\bar{o}_n$ on the right side of our equation and rearrange some more.
\begin{alignat*}{2}
    & \bar{o}_n Q_{n + 1} && = \alpha R_n + \left(\bar{o}_n - \alpha\right) Q_n \\
    \implies\quad & \bar{o}_n Q_{n + 1} && = \alpha R_n + \left[\bar{o}_{n-1} + \alpha \left(1 - \bar{o}_{n - 1}\right) - \alpha\right] Q_n \\
    & && = \alpha R_n + \left(\bar{o}_{n-1} - \alpha \bar{o}_{n - 1}\right) Q_n \\
    & && = \alpha R_n + \left(1 - \alpha \right) \bar{o}_{n - 1} Q_n
\end{alignat*}
Now we can easily substitute in the expression $Q_n$ and follow the same steps as before.
\begin{alignat*}{2}
    & \bar{o}_n Q_{n + 1} && = \alpha R_n + \left(1 - \alpha \right) \bar{o}_{n - 1} Q_n \\
    \implies\quad & \bar{o}_n Q_{n + 1} && = \alpha R_n + \left(1 - \alpha \right) \bar{o}_{n - 1} \left[Q_{n - 1} + \beta_{n - 1}\left(R_{n - 1} - Q_{n - 1}\right)\right] \\
    & && \vdots \\
    & && = \alpha R_n + \left(1 - \alpha\right) \alpha R_{n - 1} + \left(1 - \alpha\right)^2\bar{o}_{n - 2}Q_{n - 1}
\end{alignat*}
We can repeat this while process recursively until we reach $Q_1$ (our initial action value estimate).
Additionally, we can restructure our equation into a form resembling \eqref{eq:sample_average}:
\begin{equation*}
    \bar{o}_n Q_{n + 1} = \left(1 - \alpha\right)^n\bar{o}_0Q_1 + \sum^n_{i = 1}\alpha \left(1 - \alpha\right)^{n - i}R_i
    \quad\text{.}
\end{equation*}
Remember, $\bar{o}_n \doteq 0$, so we can simplify some more:
\begin{alignat*}{2}
    & \bar{o}_n Q_{n + 1} && = \left(1 - \alpha\right)^n\bar{o}_0Q_1 + \sum^n_{i = 1}\alpha \left(1 - \alpha\right)^{n - i}R_i \\
    & && = \sum^n_{i = 1}\alpha \left(1 - \alpha\right)^{n - i}R_i \\
    \implies\quad & Q_{n + 1} && = \frac{1}{\bar{o}_n} \sum^n_{i = 1}\alpha \left(1 - \alpha\right)^{n - i}R_i
    \quad\text{.}
\end{alignat*}
Finally, we have shown that $Q_{n + 1}$ is an exponential recency-weighted average without initial bias.

\end{document}
